CPSing compilation, with first serious correctness case proved, modulo universe inconsistency

platform/Depl/Compile.v
@@ -53,6 +53,19 @@ Proof.
   eauto 10.
 Qed.
 
+Theorem exprC_hygienic : forall xs vs e e' fvs,
+  exprD vs e = Some e'
+  -> exprV xs e
+  -> ~In "rp" xs
+  -> (forall x e0, vs x = Some e0
+    -> forall fE1 fE2, (forall y, In y fvs -> fE1 y = fE2 y) -> Logic.exprD e0 fE1 = Logic.exprD e0 fE2)
+  -> (forall fE1 fE2, (forall y, In y fvs -> fE1 y = fE2 y) -> Logic.exprD e' fE1 = Logic.exprD e' fE2).
+Proof.
+  destruct e; simpl; intuition eauto.
+
+  injection H; clear H; intros; subst; eauto.
+Qed.
+
 
 (** * Lowering statements *)
 
@@ -97,6 +110,28 @@ Definition precond (vs : vars) (pre post : normal) :=
       (* The postcondition holds, in an [fo_env] that lets it mention the return value. *)
       * normalD post (fo_set fE "result" (Dyn R)).
 
+(** Evaluate the arguments to a constructor, saving results in a record in memory. *)
+Fixpoint initArgs (args : list expr) (base : fo_var) (pos : nat) : chunk :=
+  match args with
+  | nil => Skip
+  | arg :: args =>
+    base + pos *<- exprC arg;;
+    initArgs args base (4 + pos)
+  end%SP.
+
+Section ForallF.
+  Variable A : Type.
+  Variables P Q : A -> Prop.
+
+  Hypothesis P_Q : forall x, P x -> Q x.
+
+  Theorem ForallF_weaken : forall ls,
+    ForallF P ls -> ForallF Q ls.
+  Proof.
+    induction ls; simpl; intuition.
+  Qed.
+End ForallF.
+
 Section stmtC.
   Variable dts : list ndatatype.
 
@@ -134,6 +169,8 @@ Section stmtC.
                             :: nil) :: lhs |} in
                         x <-- Call "malloc"!"malloc"(0, S (length args))
                         [precond vs' pre' post];;
+                        x *<- tag;;
+                        initArgs args x 4;;
                         k vs' (nextDt :: fvs) pre' post (nextDt ++ "'")%string
                     end
                 end
@@ -142,251 +179,252 @@ Section stmtC.
     end%SP.
 
 
-(** * Key lemmas to pass to Wrap *)
+  (** * Key lemmas to pass to Wrap *)
 
-Lemma vars_ok_sel : forall fE V vs,
-  vars_ok fE (sel V) vs = vars_ok fE V vs.
-Proof.
-  auto.
-Qed.
+  Lemma vars_ok_sel : forall fE V vs,
+    vars_ok fE (sel V) vs = vars_ok fE V vs.
+  Proof.
+    auto.
+  Qed.
 
-Hint Rewrite vars_ok_sel.
+  Hint Rewrite vars_ok_sel.
 
-(* Use a hypothesis telling us an expanded form implied by the known precondition. *)
-Ltac pre_implies :=
-  match goal with
-    | [ H : interp _ _, H' : forall specs0 : codeSpec _ _, _ |- _ ] =>
-      apply H' in H; clear H'; post; intuition idtac; autorewrite with core in *
-  end.
+  (* Use a hypothesis telling us an expanded form implied by the known precondition. *)
+  Ltac pre_implies :=
+    match goal with
+      | [ H : interp _ _, H' : forall specs0 : codeSpec _ _, _ |- _ ] =>
+        apply H' in H; clear H'; post; intuition idtac; autorewrite with core in *
+    end.
 
-Ltac rewriteall :=
-  repeat match goal with
-           | [ H : _ |- _ ] => rewrite H in *
-         end.
-
-(* Case-split on an [option] being [match]ed in conclusion. *)
-Ltac case_option :=
-  match goal with
-    | [ |- context[match ?E with None => _ | _ => _ end] ] =>
-      match E with
-        | context[match _ with None => _ | _ => _ end] => fail 1
-        | _ => case_eq E; post
-      end
-    | [ _ : context[match ?E with None => _ | _ => _ end] |- _ ] =>
-      match E with
-        | context[match _ with None => _ | _ => _ end] => fail 1
-        | _ => case_eq E; post; rewriteall
-      end
-    | [ _ : context[if in_dec string_dec ?x ?y then _ else _] |- _ ] =>
-      destruct (in_dec string_dec x y); post
-  end; autorewrite with core in *.
-
-(* Use a hypothesis about some fact holding for all members of a list. *)
-Ltac use_In :=
-  match goal with
-    | [ H : forall x, In x ?xs -> _ -> False, H' : In _ ?xs |- _ ] =>
-      let T := type of (H _ H') in
-        match goal with
-          | [ _ : T |- _ ] => fail 1
-          | _ => generalize (H _ H'); intro
-        end
-  end.
-
-(* Use [evaluate] to get pure facts in a precondition into the normal proof context. *)
-Ltac pre_evalu :=
-  repeat match goal with
-           | [ H : evalInstrs _ _ _ = _ |- _ ] => generalize dependent H
-           | [ H : _ _ = Some _ |- _ ] => generalize dependent H
-           | [ H : _ _ = None -> False |- _ ] => generalize dependent H
-           | [ x : _ -> option Logic.expr |- _ ] => change vars in x
-         end;
-  try match goal with
-        | [ _ : interp _ (![_] (fst ?st, _)) |- _ ] =>
-          destruct st; simpl in *
-      end; clear_fancy; evaluate auto_ext; intros.
-
-(* Clear hypotheses that will confuse Bedrock automation. *)
-Ltac cancl_clear :=
-  repeat match goal with
-           | [ H : importsGlobal _ |- _ ] => clear dependent H
-           | [ H : _ _ = Some _ |- _ ] => clear H
-           | [ H : (_ _ <> None)%type |- _ ] => clear H
-           | [ H : _ _ = None -> False |- _ ] => clear H
-           | [ H : stmtD _ _ _ _ _ |- _ ] => clear H
-         end.
-
-(* Use separation logic entailment from a hypothesis to conclusion. *)
-Ltac cancl :=
-  match goal with
-    | [ _ : interp ?specs1 (![_] (?s1, ?x1)) |- interp ?specs2 (![_] (?s2, ?x2)) ] =>
-      equate specs1 specs2; equate s1 s2; equate x1 x2;
-      cancl_clear; cancel auto_ext
-    | [ _ : interp ?specs (![_] ?s) |- interp ?specs (![_] ?s) ] =>
-      cancl_clear; cancel auto_ext
-    | [ |- interp _  (![_]%PropX _ ---> ![_]%PropX _) ] => cancl_clear; cancel auto_ext
-  end.
-
-(* Apply the [exprC_correct] lemma, using cancelation to prove one of its premises. *)
-Ltac exprC_correct :=
-  match goal with
-    | [ H : exprD _ _ = Some _ |- _ ] => eapply exprC_correct in H; try cancl; eauto;
-      try match goal with
-            | [ H : exists x, _ /\ _ |- _ ] => destruct H as [ ? [ ? [ ] ] ]
-          end
-  end.
-
-Lemma determine_rvalue : forall stn st lv rv st' w is,
-  evalInstrs stn st (IL.Assign lv rv :: is) = st'
-  -> evalRvalue stn st rv = Some w
-  -> evalInstrs stn st (IL.Assign lv w :: is) = st'.
-Proof.
-  Transparent evalInstrs.
-  simpl; intros.
-  rewrite H0 in *; auto.
-  Opaque evalInstrs.
-Qed.
-
-(* Use a previous conclusion of [exprC_correct] to simplify an [evalInstrs] hypothesis. *)
-Ltac determine_rvalue :=
-  match goal with
-    | [ H1 : evalInstrs _ _ _ = _, H2 : evalRvalue _ _ _ = Some _ |- _ ] =>
-      eapply determine_rvalue in H1; [ clear H2 | exact H2 ]
-  end.
-
-(* Full symbolic evaluation *)
-Ltac evalu :=
-  try determine_rvalue;
-    try match goal with
-          | [ H : In _ _, H' : forall x, In x _ -> In x _ |- _ ] =>
-            apply H' in H
-        end; simp;
+  Ltac rewriteall :=
     repeat match goal with
+             | [ H : _ |- _ ] => rewrite H in *
+           end.
+
+  (* Case-split on an [option] being [match]ed in conclusion. *)
+  Ltac case_option :=
+    match goal with
+      | [ |- context[match ?E with None => _ | _ => _ end] ] =>
+        match E with
+          | context[match _ with None => _ | _ => _ end] => fail 1
+          | _ => case_eq E; post
+        end
+      | [ _ : context[match ?E with None => _ | _ => _ end] |- _ ] =>
+        match E with
+          | context[match _ with None => _ | _ => _ end] => fail 1
+          | _ => case_eq E; post; rewriteall
+        end
+      | [ _ : context[if in_dec string_dec ?x ?y then _ else _] |- _ ] =>
+        destruct (in_dec string_dec x y); post
+    end; autorewrite with core in *.
+
+  (* Use a hypothesis about some fact holding for all members of a list. *)
+  Ltac use_In :=
+    match goal with
+      | [ H : forall x, In x ?xs -> _ -> False, H' : In _ ?xs |- _ ] =>
+        let T := type of (H _ H') in
+          match goal with
+            | [ _ : T |- _ ] => fail 1
+            | _ => generalize (H _ H'); intro
+          end
+    end.
+
+  (* Use [evaluate] to get pure facts in a precondition into the normal proof context. *)
+  Ltac pre_evalu :=
+    repeat match goal with
+             | [ H : evalInstrs _ _ _ = _ |- _ ] => generalize dependent H
              | [ H : _ _ = Some _ |- _ ] => generalize dependent H
              | [ H : _ _ = None -> False |- _ ] => generalize dependent H
-           end; clear_fancy;
-  (* Extra simplification for function return *)
-  try match goal with
-        | [ _ : context[locals ("rp" :: ?ns) _ _ _], H : context[natToW 0] |- _ ] =>
-          assert (In "rp" ("rp" :: ns)) by (simpl; tauto);
-            change (natToW 0) with (natToW (variablePosition ("rp" :: ns) "rp")) in H
-      end;
-  evaluate auto_ext; intros.
+             | [ x : _ -> option Logic.expr |- _ ] => change vars in x
+             | [ x : vars -> _ |- _ ] => generalize dependent x
+             | [ H : importsGlobal _ |- _ ] => generalize dependent H
+           end;
+    try match goal with
+          | [ _ : interp _ (![_] (fst ?st, _)) |- _ ] =>
+            destruct st; simpl in *
+        end; clear_fancy; evaluate auto_ext; intros.
 
-Ltac my_descend := descend; autorewrite with core in *.
-Hint Rewrite sel_upd_ne using (intro; subst; tauto).
+  (* Clear hypotheses that will confuse Bedrock automation. *)
+  Ltac cancl_clear :=
+    repeat match goal with
+             | [ H : importsGlobal _ |- _ ] => clear dependent H
+             | [ H : _ _ = Some _ |- _ ] => clear H
+             | [ H : (_ _ <> None)%type |- _ ] => clear H
+             | [ H : _ _ = None -> False |- _ ] => clear H
+             | [ H : stmtD _ _ _ _ _ |- _ ] => clear H
+           end.
 
-Lemma string_eq_complete : forall s1 s2,
-  if string_eq s1 s2 then s1 = s2 else s1 <> s2.
-Proof.
-  intros; destruct (string_dec s1 s2); subst.
-  rewrite string_eq_true; auto.
-  rewrite string_eq_false; auto.
-Qed.
+  (* Use separation logic entailment from a hypothesis to conclusion. *)
+  Ltac cancl :=
+    match goal with
+      | [ _ : interp ?specs1 (![_] (?s1, ?x1)) |- interp ?specs2 (![_] (?s2, ?x2)) ] =>
+        equate specs1 specs2; equate s1 s2; equate x1 x2;
+        cancl_clear; cancel auto_ext
+      | [ _ : interp ?specs (![_] ?s) |- interp ?specs (![_] ?s) ] =>
+        cancl_clear; cancel auto_ext
+      | [ |- interp _  (![_]%PropX _ ---> ![_]%PropX _) ] => cancl_clear; cancel auto_ext
+    end.
 
-Lemma vars_ok_upd : forall fE V vs x w e,
-  vars_ok fE V vs
-  -> Logic.exprD e fE = Dyn w
-  -> vars_ok fE (upd V x w) (vars_set vs x e).
-Proof.
-  unfold vars_ok, sel, upd, vars_set; intros.
-  generalize (string_eq_complete x0 x).
-  destruct (string_eq x0 x), (string_dec x0 x); intuition.
-Qed.
-
-Local Hint Resolve vars_ok_upd.
-
-Lemma exprV_weaken : forall xs xs',
-  (forall x, In x xs -> In x xs')
-  -> forall e, exprV xs e -> exprV xs' e.
-Proof.
-  destruct e; simpl; intuition.
-Qed.
-
-Local Hint Resolve exprV_weaken.
-
-Lemma stmtV_weaken : forall xs xs',
-  (forall x, In x xs -> In x xs')
-  -> forall s, stmtV xs s -> stmtV xs' s.
-Proof.
-  induction s; simpl; intuition eauto.
-Qed.
-
-Local Hint Resolve stmtV_weaken.
-
-Lemma vars_set_contra : forall vs x v x' v',
-  vars_set vs x v x' = None
-  -> vs x = Some v'
-  -> (vs x' = None -> False)
-  -> False.
-Proof.
-  unfold vars_set; intros;
-    destruct (string_dec x' x); subst; eauto; discriminate.
-Qed.
-
-Local Hint Resolve vars_set_contra.
-
-(* VC generation uses some empty marker predicates to indicate failure.
- * Try to find one to invert on, proving the goal trivially. *)
-Ltac use_error_message :=
-  match goal with
-    | [ H : bad_assignment_lhs _ |- _ ] => inversion H
-    | [ H : bad_assignment_rhs _ |- _ ] => inversion H
-  end.
-
-(* Use the induction hypotheses (recursively) in the proof below. *)
-Ltac Stmt_use_IH' :=
-  eauto; repeat post; my_descend; post; my_descend;
-    repeat (my_descend; cancl || (step auto_ext; my_descend)).
-
-Ltac Stmt_use_IH :=
-  match goal with
-    | [ IH : forall pre0 : _ -> _, _, H : interp _ (Structured.Postcondition _ _) |- _ ] =>
-      eapply IH in H; clear IH; auto;
+  (* Apply the [exprC_correct] lemma, using cancelation to prove one of its premises. *)
+  Ltac exprC_correct :=
+    match goal with
+      | [ H : exprD _ _ = Some _ |- _ ] => eapply exprC_correct in H; try cancl; eauto;
         try match goal with
-              | [ |- forall specs : codeSpec _ _, _ ] => intros; Stmt_use_IH
-            end; Stmt_use_IH'
-  end.
+              | [ H : exists x, _ /\ _ |- _ ] => destruct H as [ ? [ ? [ ] ] ]
+            end
+    end.
 
-Lemma addQuants_Emp : forall G (S : subs _ _ G) qs fE,
-  SubstsH S (addQuants qs (fun _ : fo_env => Emp) fE) ===> Emp.
-Proof.
-  induction qs; simpl; intros; Himp.
+  Lemma determine_rvalue : forall stn st lv rv st' w is,
+    evalInstrs stn st (IL.Assign lv rv :: is) = st'
+    -> evalRvalue stn st rv = Some w
+    -> evalInstrs stn st (IL.Assign lv w :: is) = st'.
+  Proof.
+    Transparent evalInstrs.
+    simpl; intros.
+    rewrite H0 in *; auto.
+    Opaque evalInstrs.
+  Qed.
 
-  apply Himp_refl.
+  (* Use a previous conclusion of [exprC_correct] to simplify an [evalInstrs] hypothesis. *)
+  Ltac determine_rvalue :=
+    match goal with
+      | [ H1 : evalInstrs _ _ _ = _, H2 : evalRvalue _ _ _ = Some _ |- _ ] =>
+        eapply determine_rvalue in H1; [ clear H2 | exact H2 ]
+    end.
 
-  apply Himp'_ex; auto.
-Qed.
+  (* Full symbolic evaluation *)
+  Ltac evalu :=
+    try determine_rvalue;
+      try match goal with
+            | [ H : In _ _, H' : forall x, In x _ -> In x _ |- _ ] =>
+              apply H' in H
+          end; simp;
+      repeat match goal with
+               | [ H : _ _ = Some _ |- _ ] => generalize dependent H
+               | [ H : _ _ = None -> False |- _ ] => generalize dependent H
+               | [ H : importsGlobal _ |- _ ] => generalize dependent H
+             end; clear_fancy;
+    (* Extra simplification for function return *)
+    try match goal with
+          | [ _ : context[locals ("rp" :: ?ns) _ _ _], H : context[natToW 0] |- _ ] =>
+            assert (In "rp" ("rp" :: ns)) by (simpl; tauto);
+              change (natToW 0) with (natToW (variablePosition ("rp" :: ns) "rp")) in H
+        end;
+    evaluate auto_ext; intros.
 
-Theorem sentail_sound : forall fvs fE S lhs rhs P,
-  sentail fvs lhs rhs = ProveThis P
-  -> P
-  -> List.Forall (wellScoped (NQuants rhs ++ fvs)) (NImpure rhs)
-  -> (forall x, In x fvs -> ~In x (NQuants lhs))
-  -> SubstsH S (normalD lhs fE)
-  ===> SubstsH S (normalD rhs fE).
-Proof.
-  unfold sentail; intros.
-  case_eq (cancel fvs lhs rhs); intros.
-  Focus 2.
-  rewrite H3 in *; discriminate.
-  rewrite H3 in *.
-  destruct NewLhs; try discriminate.
-  injection H; clear H; intros; subst.
-  specialize (cancel_sound fvs fE nil (fun _ _ => Emp%Sep) S _ _ _ _ H3 H0 H1).
-  unfold Logic.normalD at 3; simpl.
-  intros.
-  unfold normalD.
-  eapply Himp_trans; try apply H; clear H; auto.
-  eapply Himp_trans; [ apply Himp_star_frame; [ apply Himp_refl | ] | ].
-  apply addQuants_Emp.
-  eapply Himp_trans; [ apply Himp_star_comm | ].
-  apply Himp_star_Emp.
-Qed.
+  Ltac my_descend := descend; autorewrite with core in *.
+  Hint Rewrite sel_upd_ne using (intro; subst; tauto).
 
-Section fvs.
-  Variable fvs : list fo_var.
+  Lemma string_eq_complete : forall s1 s2,
+    if string_eq s1 s2 then s1 = s2 else s1 <> s2.
+  Proof.
+    intros; destruct (string_dec s1 s2); subst.
+    rewrite string_eq_true; auto.
+    rewrite string_eq_false; auto.
+  Qed.
 
-  Lemma use_hygiene : forall vs x x' e0 e2 fE1 fE2,
+  Lemma vars_ok_upd : forall fE V vs x w e,
+    vars_ok fE V vs
+    -> Logic.exprD e fE = Dyn w
+    -> vars_ok fE (upd V x w) (vars_set vs x e).
+  Proof.
+    unfold vars_ok, sel, upd, vars_set; intros.
+    generalize (string_eq_complete x0 x).
+    destruct (string_eq x0 x), (string_dec x0 x); intuition.
+  Qed.
+
+  Local Hint Resolve vars_ok_upd.
+
+  Lemma exprV_weaken : forall xs xs',
+    (forall x, In x xs -> In x xs')
+    -> forall e, exprV xs e -> exprV xs' e.
+  Proof.
+    destruct e; simpl; intuition.
+  Qed.
+
+  Local Hint Resolve exprV_weaken.
+
+  Lemma stmtV_weaken : forall xs xs',
+    (forall x, In x xs -> In x xs')
+    -> forall s, stmtV dts xs s -> stmtV dts xs' s.
+  Proof.
+    induction s; simpl; intuition eauto using ForallF_weaken.
+  Qed.
+
+  Local Hint Resolve stmtV_weaken.
+
+  Lemma vars_set_contra : forall vs x v x' v',
+    vars_set vs x v x' = None
+    -> vs x = Some v'
+    -> (vs x' = None -> False)
+    -> False.
+  Proof.
+    unfold vars_set; intros;
+      destruct (string_dec x' x); subst; eauto; discriminate.
+  Qed.
+
+  Local Hint Resolve vars_set_contra.
+
+  (* VC generation uses some empty marker predicates to indicate failure.
+   * Try to find one to invert on, proving the goal trivially. *)
+  Ltac use_error_message :=
+    match goal with
+      | [ H : bad_assignment_lhs _ |- _ ] => inversion H
+      | [ H : bad_assignment_rhs _ |- _ ] => inversion H
+    end.
+
+  (* Use the induction hypotheses (recursively) in the proof below. *)
+  Ltac Stmt_use_IH' :=
+    eauto; repeat post; my_descend; post; my_descend;
+      repeat (my_descend; cancl || (step auto_ext; my_descend)).
+
+  Ltac Stmt_use_IH :=
+    match goal with
+      | [ IH : forall pre0 : _ -> _, _, H : interp _ (Structured.Postcondition _ _) |- _ ] =>
+        eapply IH in H; clear IH; auto;
+          try match goal with
+                | [ |- forall specs : codeSpec _ _, _ ] => intros; Stmt_use_IH
+              end; Stmt_use_IH'
+    end.
+
+  Lemma addQuants_Emp : forall G (S : subs _ _ G) qs fE,
+    SubstsH S (addQuants qs (fun _ : fo_env => Emp) fE) ===> Emp.
+  Proof.
+    induction qs; simpl; intros; Himp.
+
+    apply Himp_refl.
+
+    apply Himp'_ex; auto.
+  Qed.
+
+  Theorem sentail_sound : forall fvs fE S lhs rhs P,
+    sentail fvs lhs rhs = ProveThis P
+    -> P
+    -> List.Forall (wellScoped (NQuants rhs ++ fvs)) (NImpure rhs)
+    -> (forall x, In x fvs -> ~In x (NQuants lhs))
+    -> SubstsH S (normalD lhs fE)
+    ===> SubstsH S (normalD rhs fE).
+  Proof.
+    unfold sentail; intros.
+    case_eq (cancel fvs nil lhs rhs); intros.
+    Focus 2.
+    rewrite H3 in *; discriminate.
+    rewrite H3 in *.
+    destruct NewLhs; try discriminate.
+    injection H; clear H; intros; subst.
+    assert (Heasy : forall x, In x fvs -> ~In x nil) by (simpl; tauto).
+    specialize (cancel_sound fvs nil fE nil (fun _ _ => Emp%Sep) S _ _ _ _ _ Heasy H3 H0 H1).
+    unfold Logic.normalD at 3; simpl.
+    intros.
+    unfold normalD.
+    eapply Himp_trans; try apply H; clear H; auto.
+    eapply Himp_trans; [ apply Himp_star_frame; [ apply Himp_refl | ] | ].
+    apply addQuants_Emp.
+    eapply Himp_trans; [ apply Himp_star_comm | ].
+    apply Himp_star_Emp.
+  Qed.
+
+  Lemma use_hygiene : forall fvs vs x x' e0 e2 fE1 fE2,
     (forall x e, vs x = Some e
       -> forall fE1 fE2, (forall y, In y fvs -> fE1 y = fE2 y)
         -> Logic.exprD e fE1 = Logic.exprD e fE2)
@@ -403,35 +441,32 @@ Section fvs.
 
   Hint Immediate use_hygiene.
 
-  Lemma Stmt_post : forall pre post im mn (H : importsGlobal im) ns res xs,
-    ~In "rp" ns
-    -> (forall x, In x xs -> In x ns)
-    -> forall s pre0 k,
-      (forall specs st,
-        interp specs (pre0 st)
-        -> exists vs, interp specs (precond vs pre post true (fun x => x) ns res st)
-          /\ stmtD pre post fvs xs vs s k
-          /\ (forall x e, vs x = Some e
-            -> forall fE1 fE2, (forall y, In y fvs -> fE1 y = fE2 y)
-              -> Logic.exprD e fE1 = Logic.exprD e fE2))
-      -> stmtV xs s
-      -> forall specs st, interp specs (Structured.Postcondition (toCmd (stmtC s) mn H ns res pre0) st)
-        -> exists vs', k vs'
-          /\ interp specs (precond vs' pre post true (fun x => x) ns res st)
-          /\ (forall x e, vs' x = Some e
-            -> forall fE1 fE2, (forall y, In y fvs -> fE1 y = fE2 y)
-              -> Logic.exprD e fE1 = Logic.exprD e fE2).
+  (* Prove we never run off the end of a function.
+   * We're in CPS, so all postconditions should be contradictory. *)
+  Theorem stmtC_post : forall im mn (H : importsGlobal im) ns res s k,
+    (forall specs st vs fvs pre post nextDt pre0,
+       interp specs (Structured.Postcondition (toCmd (k vs fvs pre post nextDt)
+                                                     mn H ns res pre0) st)
+       -> False)
+    -> (forall specs st vs fvs pre post nextDt pre0,
+       interp specs (Structured.Postcondition (toCmd (stmtC vs fvs pre post nextDt s k)
+                                                     mn H ns res pre0) st)
+       -> False).
   Proof.
-    induction s; (repeat post; intuition;
-      repeat (pre_implies || use_In || case_option); try use_error_message; try Stmt_use_IH;
-        try (pre_evalu; exprC_correct); evalu;
-          my_descend; eauto; propxFo;
-            my_descend; repeat (my_descend; cancl || (step auto_ext; my_descend))).
+    induction s; simpl; intuition idtac;
+      repeat match goal with
+               | [ _ : context[match ?E with _ => _ end] |- _ ] =>
+                 destruct E; simpl in *; eauto
+               | [ IH : forall k : _ -> _, _, H : interp _ (Structured.Postcondition _ _) |- _ ] =>
+                 apply IH in H; clear IH; intuition idtac
+               | [ H : interp _ [| False |]%PropX |- _ ] => propxFo
+               | [ x : (_ * _)%type |- _ ] => destruct x
+             end.
   Qed.
 
   Definition normalWf' := normalWf.
 
-  Definition scopey post := List.Forall (wellScoped (NQuants post ++ "result" :: fvs)).
+  Definition scopey fvs post := List.Forall (wellScoped (NQuants post ++ "result" :: fvs)).
   Definition scopey' x := List.Forall (fun p => exists bvs, boundVars p = Some bvs /\ ~In x bvs).
 
   Theorem nsubst_bwd : forall x e fvs n fE,
@@ -449,92 +484,83 @@ Section fvs.
     eapply nsubst_bwd; eauto.
   Qed.
 
-  Lemma Stmt_vc : forall pre post im mn (H : importsGlobal im) ns res xs,
-    normalWf' fvs pre
-    -> normalWf' ("result" :: fvs) post
-    -> ~In "rp" ns
+  Lemma Stmt_vc : forall im mn (H : importsGlobal im) ns res xs,
+    ~In "rp" ns
     -> (forall x, In x xs -> In x ns)
-    -> ~In "result" fvs
-    -> ~In "result" (NQuants pre)
-    -> ~In "result" (NQuants post)
-    -> scopey post (NImpure post)
-    -> scopey' "result" (NImpure pre)
-    -> (forall x, In x fvs -> ~In x (NQuants pre))
-    -> (forall x, In x fvs -> ~In x (NQuants post))
-    -> forall s pre0 k,
-      (forall specs st,
+    -> forall s vs fvs pre post nextDt kC pre0 kD,
+      ~In "result" fvs
+      -> normalWf' fvs pre
+      -> normalWf' ("result" :: fvs) post
+      -> ~In "result" (NQuants pre)
+      -> ~In "result" (NQuants post)
+      -> scopey fvs post (NImpure post)
+      -> scopey' "result" (NImpure pre)
+      -> (forall x, In x fvs -> ~In x (NQuants pre))
+      -> (forall x, In x fvs -> ~In x (NQuants post))
+      -> stmtD dts xs vs fvs pre post nextDt s kD
+      -> (forall x e, vs x = Some e
+        -> forall fE1 fE2, (forall y, In y fvs -> fE1 y = fE2 y)
+          -> Logic.exprD e fE1 = Logic.exprD e fE2)
+      -> (forall specs st,
         interp specs (pre0 st)
-        -> exists vs, interp specs (precond vs pre post true (fun x => x) ns res st)
-          /\ stmtD pre post fvs xs vs s k
-          /\ (forall x e, vs x = Some e
-            -> forall fE1 fE2, (forall y, In y fvs -> fE1 y = fE2 y)
-              -> Logic.exprD e fE1 = Logic.exprD e fE2))
-      -> stmtV xs s
-      -> vcs (VerifCond (toCmd (stmtC s) mn H ns res pre0)).
+        -> interp specs (precond vs pre post true (fun x => x) ns res st))
+      -> (forall vs fvs pre post nextDt pre0,
+        kD vs fvs pre post nextDt
+        -> (forall x e, vs x = Some e
+          -> forall fE1 fE2, (forall y, In y fvs -> fE1 y = fE2 y)
+            -> Logic.exprD e fE1 = Logic.exprD e fE2)
+        -> (forall specs st,
+          interp specs (pre0 st)
+          -> interp specs (precond vs pre post true (fun x => x) ns res st))
+        -> vcs (VerifCond (toCmd (kC vs fvs pre post nextDt) mn H ns res pre0)))
+      -> stmtV dts xs s
+      -> vcs (VerifCond (toCmd (stmtC vs fvs pre post nextDt s kC) mn H ns res pre0)).
   Proof.
     induction s.
 
-    Ltac t := wrap0; repeat (pre_implies || use_In || case_option); simpl in *; intuition eauto;
-      try (pre_evalu; exprC_correct); try evalu;
-        try match goal with
-              | [ IH : _ |- _ ] => eapply IH; eauto; intros;
-                match goal with
-                  | [ H : interp _ _ |- _ ] => eapply Stmt_post in H;
-                    Stmt_use_IH'; (cbv beta in *; eauto)
-                end
-            end.
-
-    t.
-
-    t.
-
-    wrap0; repeat (pre_implies || use_In || case_option); simpl in *; intuition eauto;
-      try (pre_evalu; exprC_correct); try evalu.
-
-    case_eq (sentail fvs pre (nsubst "result" e0 post)); intros.
-    Focus 2.
-    rewrite H23 in *; inversion H11.
-    rewrite H23 in *.
+    wrap0.
+    simpl in *; intuition idtac.
+    case_option.
+    wrap0.
+    pre_implies.
+    simpl in *; intuition eauto.
+    pre_evalu.
+    exprC_correct.
+    evalu.
+    rewriteall.
+    case_option.
+    apply H14; intuition idtac.
+    unfold vars_set in H18.
+    destruct (string_dec x0 x); subst.
+    injection H18; clear H18; intros; subst; eauto.
+    eauto using exprC_hygienic.
+    eauto.
+    propxFo.
+    pre_implies.
+    pre_evalu.
+    exprC_correct.
+    evalu.
     descend.
+    rewrite vars_ok_sel.
+    cancl_clear.
     step auto_ext.
-    step auto_ext.
-    descend.
-    cancl.
-    specialize (sentail_sound fvs (fo_set x1 "result" (Dyn (Regs st Rv))) (@SNil _ _) _ _ _ H23); intuition.
-    unfold SubstsH in *; simpl in *.
-    eapply Himp_trans; [ | eapply nsubst_bwd; eauto ].
-    eapply Himp_trans; [ | apply H22 ].
+    descend; step auto_ext.
+    descend; step auto_ext.
+    descend; step auto_ext.
+    descend; step auto_ext.
+    descend; step auto_ext.
+    rewriteall.
+    use_error_message.
 
-    eapply weaken_normalD; eauto.
-    intros.
-    unfold fo_set.
-    destruct (string_dec x5 "result"); subst; tauto.
-    2: eauto.
-    3: simpl; unfold not; intuition (subst; eauto).
-    4: simpl; tauto.
+    admit.
+    
+    admit.
 
-    Focus 2.
-    unfold fo_set at 1; simpl.
-    etransitivity; try (symmetry; apply H13).
-    apply H14.
-    unfold fo_set; intros.
-    destruct (string_dec y "result"); subst; eauto; exfalso; eauto.
-
-    2: simpl; eauto.
-
-    eapply Forall_forall; intros.
-    eapply in_map_iff in H20; destruct H20; intuition subst.
-    eapply Forall_forall in H25; try apply H7.
-
-    eapply wellScoped_psubst.
-    eapply wellScoped_weaken; eauto.
-    simpl; intuition idtac.
-    apply in_app_or in H; intuition eauto using in_or_app.
-    simpl in *; intuition eauto using in_or_app.
-    eauto using in_or_app.
+    admit.
   Qed.
 End fvs.
 
+(*
 Local Hint Immediate wellScoped_predExt.
 
 Lemma scopey_normalize : forall fvs post post' bvs',
@@ -627,3 +653,4 @@ Proof.
                                eauto 6 ]
                            end) ].
 Defined.
+*)
